Updates.

FOL/Parsing/EpsilonNFA.lean
@@ -33,7 +33,6 @@ structure EpsilonNFA
   deriving Repr
 
 
-@[simp]
 def epsilon_arrow_list_to_graph
   {σ : Type} :
   List (EpsilonArrow σ) → Graph σ
@@ -41,7 +40,6 @@ def epsilon_arrow_list_to_graph
   | (hd :: tl) => (hd.start_state, hd.stop_state_list) :: epsilon_arrow_list_to_graph tl
 
 
-@[simp]
 def EpsilonNFA.epsilon_closure
   {α : Type}
   {σ : Type}
@@ -55,7 +53,6 @@ def EpsilonNFA.epsilon_closure
 /--
   The accumulated stop states of all of the arrows in the list that have a start state and symbol matching the given state and symbol.
 -/
-@[simp]
 def symbol_arrow_list_to_fun
   {α : Type}
   [DecidableEq α]
@@ -95,7 +92,6 @@ example : symbol_arrow_list_to_fun [⟨0, 'a', [1]⟩, ⟨0, 'a', [1]⟩, ⟨0, 
 /--
   `EpsilonNFA.eval_one e l c` := Returns the list of states that the nondeterministic automaton `e` transitions to if it starts at the list of states `l` and consumes the symbol `c`.
 -/
-@[simp]
 def EpsilonNFA.eval_one
   {α : Type}
   [DecidableEq α]
@@ -108,7 +104,6 @@ def EpsilonNFA.eval_one
   e.epsilon_closure (state_list.map (fun (state : σ) => (symbol_arrow_list_to_fun e.symbol_arrow_list) state symbol)).join.dedup
 
 
-@[simp]
 def EpsilonNFA.eval_from
   {α : Type}
   [DecidableEq α]
@@ -121,7 +116,6 @@ def EpsilonNFA.eval_from
   List.foldl e.eval_one (e.epsilon_closure starting_state_list) input
 
 
-@[simp]
 def EpsilonNFA.eval
   {α : Type}
   [DecidableEq α]
@@ -133,7 +127,6 @@ def EpsilonNFA.eval
   e.eval_from e.starting_state_list input
 
 
-@[simp]
 def EpsilonNFA.accepts
   {α : Type}
   [DecidableEq α]
@@ -184,3 +177,222 @@ example : EpsilonNFA.eval ⟨ [⟨0, 'a', [1]⟩, ⟨0, 'a', [2]⟩], [], [0], [
 example : EpsilonNFA.eval ⟨ [], [⟨ 0, [1] ⟩], [0], [1] ⟩ ([] : List Char) = [1, 0] := by rfl
 
 example : EpsilonNFA.eval ⟨ [], [⟨ 0, [1]⟩], [0], [1] ⟩ ['a'] = [] := by rfl
+
+
+-------------------------------------------------------------------------------
+
+
+structure AbstractEpsilonNFA
+  (α : Type)
+  (σ : Type) :
+  Type :=
+  (symbol : σ → α → σ → Prop)
+  (epsilon : σ → σ → Prop)
+  (start : σ → Prop)
+  (accepting : σ → Prop)
+
+
+inductive AbstractEpsilonNFA.Eval
+  {α σ : Type}
+  (M : AbstractEpsilonNFA α σ) :
+  σ → List α → Prop
+  | eps
+    {s s' : σ}
+    {as : List α} :
+    M.epsilon s s' →
+    Eval M s' as →
+    Eval M s as
+
+  | sym
+    {s s' : σ}
+    {a : α}
+    {as : List α} :
+    M.symbol s a s' →
+    Eval M s' as →
+    Eval M s (a :: as)
+
+  | accept
+    {s : σ} :
+    M.accepting s →
+    Eval M s []
+
+
+def AbstractEpsilonNFA.Accepts
+  {α : Type}
+  {σ : Type}
+  (M : AbstractEpsilonNFA α σ)
+  (as : List α) :
+  Prop :=
+  ∃ (s : σ), M.start s ∧ M.Eval s as
+
+
+def EpsilonNFA.toAbstract
+  {α : Type}
+  {σ : Type}
+  (M : EpsilonNFA α σ) :
+  AbstractEpsilonNFA α σ :=
+  {
+    symbol := fun (start_state : σ) (symbol : α) (stop_state : σ) => ∃ (stop_state_list : List σ), ⟨start_state, symbol, stop_state_list⟩ ∈ M.symbol_arrow_list ∧ stop_state ∈ stop_state_list,
+
+    epsilon := fun (start_state : σ) (stop_state : σ) => ∃ (stop_state_list : List σ), ⟨start_state, stop_state_list⟩ ∈ M.epsilon_arrow_list ∧ stop_state ∈ stop_state_list,
+
+    start := fun (s : σ) => s ∈ M.starting_state_list,
+
+    accepting := fun (s : σ) => s ∈ M.accepting_state_list
+  }
+
+
+def EpsilonNFA.eval_one'
+  {α : Type}
+  [DecidableEq α]
+  {σ : Type}
+  [DecidableEq σ]
+  (e : EpsilonNFA α σ)
+  (state_list : List σ)
+  (symbol : α) :
+  List σ :=
+  (state_list.map (fun (state : σ) => (symbol_arrow_list_to_fun e.symbol_arrow_list) state symbol)).join.dedup
+
+
+theorem EpsilonNFA.eval_one'_def
+  {α : Type} [DecidableEq α] {σ : Type} [DecidableEq σ]
+  (e : EpsilonNFA α σ)
+  (state_list : List σ)
+  (symbol : α) {s} :
+  s ∈ e.eval_one' state_list symbol ↔
+  (∃ a ∈ state_list, s ∈ symbol_arrow_list_to_fun e.symbol_arrow_list a symbol) := by simp [eval_one']
+
+
+theorem EpsilonNFA.eval_one'_iff {α σ} [DecidableEq α] [DecidableEq σ]
+    (M : EpsilonNFA α σ) {S s' a} :
+    s' ∈ M.eval_one' S a ↔ (∃ s ∈ S, M.toAbstract.symbol s a s') := by
+  simp [eval_one', toAbstract, symbol_arrow_list_to_fun]
+  constructor
+  · rintro ⟨_, h1, _, ⟨⟨⟩, h2, ⟨rfl, rfl⟩, rfl⟩, h3⟩
+    exact ⟨_, h1, _, h2, h3⟩
+  · rintro ⟨_, h1, _, h2, h3⟩
+    exact ⟨_, h1, _, ⟨_, h2, ⟨rfl, rfl⟩, rfl⟩, h3⟩
+
+
+@[simp]
+theorem EpsilonNFA.eval_from_nil
+  {α : Type} [DecidableEq α] {σ : Type} [DecidableEq σ]
+  (e : EpsilonNFA α σ) (S : List σ) :
+  e.eval_from S [] = e.epsilon_closure S := rfl
+
+@[simp]
+theorem EpsilonNFA.eval_from_cons
+  {α : Type} [DecidableEq α] {σ : Type} [DecidableEq σ]
+  (e : EpsilonNFA α σ) (S : List σ) (a as) :
+  e.eval_from S (a :: as) = e.eval_from (e.eval_one' (e.epsilon_closure S) a) as := rfl
+
+
+abbrev AbstractEpsilonNFA.EpsilonClosure {α σ} (M : AbstractEpsilonNFA α σ) :=
+  Relation.ReflTransGen M.epsilon
+
+
+theorem EpsilonNFA.epsilon_closure_iff
+  {α : Type} [DecidableEq α] {σ : Type} [DecidableEq σ]
+  (e : EpsilonNFA α σ) {S s'} :
+  s' ∈ e.epsilon_closure S ↔ ∃ s ∈ S, e.toAbstract.EpsilonClosure s s' := by
+  simp [epsilon_closure, dft_iff]
+  congr! with a b c
+  simp [toAbstract]
+  induction e.epsilon_arrow_list <;> simp [*, epsilon_arrow_list_to_graph, or_and_right, exists_or]
+  apply or_congr_left <| exists_congr fun a => and_congr_left fun _ => ?_
+  constructor <;> [rintro ⟨rfl, rfl⟩; rintro rfl] <;> [rfl; constructor <;> rfl]
+
+
+theorem EpsilonNFA.eval_from_iff {α σ} [DecidableEq α] [DecidableEq σ]
+    (M : EpsilonNFA α σ) {S input} :
+    (∃ s ∈ M.eval_from S input, s ∈ M.accepting_state_list) ↔
+    (∃ s ∈ S, M.toAbstract.Eval s input) := by
+  induction input generalizing S with simp
+  | nil =>
+    simp [epsilon_closure_iff]
+    constructor
+    · intro ⟨s, ⟨s', h1, h2⟩, h3⟩
+      refine ⟨_, h1, ?_⟩
+      clear h1
+      induction h2 using Relation.ReflTransGen.head_induction_on with
+      | refl => exact .accept h3
+      | head h _ ih => exact .eps h ih
+    · intro ⟨s, h1, h2⟩
+      obtain ⟨s', h3, h4⟩ : ∃ s', M.toAbstract.EpsilonClosure s s' ∧ s' ∈ M.accepting_state_list := by
+        clear h1; generalize e : [] = l at h2
+        induction h2 with cases e
+        | accept h' => exact ⟨_, .refl, h'⟩
+        | eps h1 _ ih =>
+          have ⟨s', h3, h4⟩ := ih rfl
+          exact ⟨_, .head h1 h3, h4⟩
+      exact ⟨_, ⟨_, h1, h3⟩, h4⟩
+  | cons a as IH =>
+    simp [IH, epsilon_closure_iff, eval_one'_iff]
+    constructor
+    · intro ⟨s₁, ⟨s₂, ⟨s₃, h1, h2⟩, h3⟩, h4⟩
+      refine ⟨_, h1, ?_⟩
+      clear h1
+      induction h2 using Relation.ReflTransGen.head_induction_on with
+      | refl => exact .sym h3 h4
+      | head h _ ih => exact .eps h ih
+    · intro ⟨s, h1, h2⟩
+      obtain ⟨s₁, s₂, h3, h4, h5⟩ :
+          ∃ s₁ s₂, M.toAbstract.EpsilonClosure s s₂ ∧
+            M.toAbstract.symbol s₂ a s₁ ∧ M.toAbstract.Eval s₁ as := by
+        clear h1; generalize e : a::as = l at h2
+        induction h2 with cases e
+        | sym h1 h2 => exact ⟨_, _, .refl, h1, h2⟩
+        | eps h1 _ ih =>
+          have ⟨s₁, s₂, h3, h4, h5⟩ := ih rfl
+          exact ⟨_, _, .head h1 h3, h4, h5⟩
+      exact ⟨_, ⟨_, ⟨_, h1, h3⟩, h4⟩, h5⟩
+
+
+theorem EpsilonNFA.accepts_iff {α σ} [DecidableEq α] [DecidableEq σ]
+    (M : EpsilonNFA α σ) {input} : M.accepts input ↔ M.toAbstract.Accepts input := by
+  simp [accepts, eval]; rw [EpsilonNFA.eval_from_iff]; rfl
+
+
+
+
+
+
+
+def EpsilonNFA.map
+  {α : Type}
+  {σ₁ σ₂ : Type}
+  (f : σ₁ → σ₂)
+  (e : EpsilonNFA α σ₁) :
+  EpsilonNFA α σ₂ :=
+  {
+    symbol_arrow_list := e.symbol_arrow_list.map (fun (arrow : SymbolArrow α σ₁) => ⟨
+      f arrow.start_state,
+      arrow.symbol,
+      arrow.stop_state_list.map f
+    ⟩),
+    epsilon_arrow_list := e.epsilon_arrow_list.map (fun (arrow : EpsilonArrow σ₁) => ⟨
+      f arrow.start_state,
+      arrow.stop_state_list.map f
+    ⟩),
+    starting_state_list := e.starting_state_list.map f,
+    accepting_state_list := e.accepting_state_list.map f
+  }
+
+
+def AbstractEpsilonNFA.map
+  {α : Type}
+  {σ₁ σ₂ : Type}
+  (f_inv : σ₂ → σ₁)
+  (e : AbstractEpsilonNFA α σ₁) :
+  AbstractEpsilonNFA α σ₂ :=
+  {
+    symbol := fun (start_state : σ₂) (symbol : α) (stop_state: σ₂) =>
+    (e.symbol (f_inv start_state) symbol (f_inv stop_state)),
+
+    epsilon := fun (start_state : σ₂) (stop_state: σ₂) =>
+    (e.epsilon (f_inv start_state) (f_inv stop_state)),
+
+    start := fun (state : σ₂) => e.start (f_inv state),
+
+    accepting := fun (state : σ₂) => e.accepting (f_inv state)
+  }
